\documentclass{article}
\usepackage{amsmath}
\usepackage{parskip}
\usepackage{lmodern}
\begin{document}
After substituting I17 into I16 we get
\begin{equation}
    \mathcal{V}^{S,a,\ell}_{nm} = 
    \frac{i\Sigma}{2}\sum_{q}\left(f_{qn}r^{a}_{nq}C^{\ell}_{qm}
                                 + f_{mq}C^{\ell}_{nq}r^{a}_{qm}\right),
    \end{equation}
where $f_{mn} = f_{m} - f_{n}$ and $f_{mn} = -f_{nm}$. For a clean cold 
semiconductor, $f_{n} = 1$ for an occupied or valence $(n = v)$ band, 
and $f_{n} = 0$ for an empty or conduction $(n = c)$ band.

There are four cases:
\begin{enumerate}
\item Valence $\rightarrow$ Conduction: 
  For $nm = vc$, we have
  \begin{equation}\label{conval}
    \mathcal{V}^{S,a,\ell}_{vc} = 
    \frac{i\Sigma}{2}
    \sum_{q}\left(f_{qv}r^{a}_{vq}C^{\ell}_{qc}
                + f_{cq}C^{\ell}_{vq}r^{a}_{qc}\right).
  \end{equation}
  $f_{qv} = 0$ for every valence state ($q = v$). 
  For conduction states ($q = c$),
  \begin{equation*}
      f_{cv} = f_{c} - f_{v} = 0 - 1 = -1.
  \end{equation*}
  Likewise, $f_{cq} = 0$ for all conduction states, and $f_{cv} = -1$ 
  for valence states. Substituting these values in \eqref{conval} we obtain
  \begin{equation}
      \mathcal{V}^{S,a,\ell}_{vc} = 
      -\frac{i\Sigma}{2}
      \left[\sum_{c^{\prime}}r^{a}_{vc^{\prime}}C^{\ell}_{c^{\prime}c}
          + \sum_{v^{\prime}}C^{\ell}_{vv^{\prime}}r^{a}_{v^{\prime}c}\right].
  \end{equation}

\item Conduction $\rightarrow$ Valence:
  For $nm = cv$, we have
  \begin{equation}\label{valcon}
    \mathcal{V}^{S,a,\ell}_{cv} = 
    \frac{i\Sigma}{2}
    \sum_{q}\left(f_{qc}r^{a}_{cq}C^{\ell}_{qv} 
                + f_{vq}C^{\ell}_{cq}r^{a}_{qv}\right).
  \end{equation}
  $f_{qc} = 0$ for every conduction state ($q = c$). 
  For valence states ($q = v$),
  \begin{equation*}
      f_{vc} = f_{v} - f_{c} = 1 - 0 = 1.
  \end{equation*}
  Likewise, $f_{vq} = 0$ for all valence states, and $f_{vc} = 1$ 
  for conduction states. Substituting these values in \eqref{valcon} we obtain
  \begin{equation}
      \mathcal{V}^{S,a,\ell}_{cv} = 
      \frac{i\Sigma}{2}
      \left[\sum_{v^{\prime}}r^{a}_{cv^{\prime}}C^{\ell}_{v^{\prime}v} 
          + \sum_{c^{\prime}}C^{\ell}_{cc^{\prime}}r^{a}_{c^{\prime}v}\right].
  \end{equation}

\item Valence $\rightarrow$ Valence:
  For $n = m = v$, we have
  \begin{equation}\label{valval}
    \mathcal{V}^{S,a,\ell}_{vv} = 
    \frac{i\Sigma}{2}\sum_{q}
    \left(f_{qv}r^{a}_{vq}C^{\ell}_{qv} 
        + f_{vq}C^{\ell}_{vq}r^{a}_{qv}\right).
  \end{equation}
  $f_{qv} = f_{vq}= 0$ for every valence state ($q = v$). 
  For conduction states ($q = c$),
  \begin{align*}
      f_{cv} &= f_{c} - f_{v} = -1,\\
      f_{vc} &= -f_{cv} = 1.
  \end{align*}
  Substituting these values in \eqref{valval} we obtain
  \begin{align}
    \mathcal{V}^{S,a,\ell}_{vv} 
    &= \frac{i\Sigma}{2}\sum_{c^{\prime}}
    -\left(r^{a}_{vc^{\prime}}C^{\ell}_{c^{\prime}v} 
         - C^{\ell}_{vc^{\prime}}r^{a}_{c^{\prime}v}\right)\nonumber\\
    &= \frac{\Sigma}{2}\sum_{c^{\prime}}
    -i\left[r^{a}_{vc^{\prime}}C^{\ell}_{c^{\prime}v} 
       - (r^{a}_{vc^{\prime}}C^{\ell}_{c^{\prime}v})^{*}\right]\nonumber\\
    &= \Sigma\sum_{c^{\prime}}
    \text{Im}\left[r^{a}_{vc^{\prime}}C^{\ell}_{c^{\prime}v}\right]
  \end{align}

\item Conduction $\rightarrow$ Conduction:
  For $n = m = c$, we have
  \begin{equation}\label{concon}
    \mathcal{V}^{S,a,\ell}_{cc} = 
    \frac{i\Sigma}{2}\sum_{q}
    \left(f_{qc}r^{a}_{cq}C^{\ell}_{qc}
        + f_{cq}C^{\ell}_{cq}r^{a}_{qc}\right).
  \end{equation}
  $f_{qc} = f_{cq}= 0$ for every conduction state ($q = c$). 
  For valence states ($q = v$),
  \begin{align*}
      f_{vc} &= f_{v} - f_{c} = 1,\\
      f_{cv} &= -f_{vc} = -1.
  \end{align*}
  Substituting these values in \eqref{concon} we obtain
  \begin{align}
    \mathcal{V}^{S,a,\ell}_{cc} 
    &= \frac{i\Sigma}{2}\sum_{v^{\prime}}
    \left(r^{a}_{cv^{\prime}}C^{\ell}_{v^{\prime}c} 
        - C^{\ell}_{cv^{\prime}}r^{a}_{v^{\prime}c}\right)\nonumber\\
    &= \frac{\Sigma}{2}\sum_{v^{\prime}}
    i\left[r^{a}_{cv^{\prime}}C^{\ell}_{v^{\prime}c} 
       - (r^{a}_{cv^{\prime}}C^{\ell}_{v^{\prime}c})^{*}\right]\nonumber\\
    &= -\Sigma\sum_{v^{\prime}}
    \text{Im}\left[r^{a}_{cv^{\prime}}C^{\ell}_{v^{\prime}c}\right]
  \end{align}
\end{enumerate}

\end{document}
