\section{Matrix elements of 
\texorpdfstring{$\bfv^\nl_{nm}(\bfk)$}{Vnonlocal}
and
\texorpdfstring{$\calbv^{\nl,\ell}_{nm}(\bfk)$}{Vnonlocal}
}\label{appvnl}
From Eq.~\eqref{conhr}, we have that
\begin{align}\label{vnln.0}
\bfv^\nl_{nm}(\bfk)=\bra{n\bfk}\hat\bfv^\nl\ket{m\bfk'}
&=
\frac{i}{\hbar}
\bra{n\bfk}[\hat V^\nl,\hat\bfr]\ket{m\bfk'}
\nonumber\\
&=
\frac{i}{\hbar}
\int d\bfr d\bfr'
\braket{n\bfk}{\bfr}
\bra{\bfr}
[\hat V^\nl,\hat \bfr]
\ket{\bfr'}
\braket{\bfr'}{m\bfk'}
\nonumber\\
&=
\frac{i}{\hbar}
\gd(\bfk-\bfk')
\int d\bfr d\bfr'
\psi^*_{n\bfk}(\bfr)
\bra{\bfr}
[\hat V^\nl,\hat \bfr]
\ket{\bfr'}
\psi_{m\bfk'}(\bfr')
,
\end{align}   
where due to the fact that the integrand is periodic in real space,
$\bfk=\bfk'$ where $\bfk$ is restricted to the Brillouin Zone.
Now,
\begin{align}\label{vnln.1}
\bra{\bfr}
[\hat V^\nl,\hat \bfr]
\ket{\bfr'}
&=
\bra{\bfr}
\hat V^\nl\hat \bfr
-
\hat \bfr\hat V^\nl
\ket{\bfr'}
=
\bra{\bfr}
\hat V^\nl\hat \bfr
\ket{\bfr'}
-
\bra{\bfr}
\hat \bfr\hat V^\nl
\ket{\bfr'}
\nonumber\\
&=
\bra{\bfr}
\hat V^\nl \bfr'
\ket{\bfr'}
-
\bra{\bfr}
\bfr\hat V^\nl
\ket{\bfr'}
=
\bra{\bfr}
\hat V^\nl
\ket{\bfr'}
\big(\bfr'-\bfr\big)
=V^\nl(\bfr,\bfr') \big(\bfr'-\bfr\big)
,
\end{align}
where we use 
$\hat r \bra{\bfr}=r \bra{\bfr}$,
$\bra{\bfr'}\hat r=\bra{\bfr}r'$,
and $V^\nl(\bfr,\bfr')=\bra{\bfr}\hat V^\nl\ket{\bfr'}$ (Eq.~\eqref{ache.3n}).
Also, we have the following identity which will be used shortly, 
\begin{align}\label{cn51}
(\nabla_\bfK+\nabla_{\bfK'})
\frac{1}{\gO}
\int e^{-i\bfK\cdot\bfr}
V^\nl(\bfr,\bfr')
e^{i\bfK'\cdot\bfr'}
\,d\bfr d\bfr'
&=
-i
\frac{1}{\gO}
\int e^{-i\bfK\cdot\bfr}
\left(
\bfr
V^\nl(\bfr,\bfr')
-
V^\nl(\bfr,\bfr')
\bfr'
\right)
e^{i\bfK'\cdot\bfr'}
\,d\bfr d\bfr'
\nonumber\\
(\nabla_\bfK+\nabla_{\bfK'})
\bra{\bfK}
V^\nl
\ket{\bfK'}
&=
\frac{i}{\gO}
\int e^{-i\bfK\cdot\bfr}
V^\nl(\bfr,\bfr')
\big(
\bfr'
-
\bfr
\big)
e^{i\bfK'\cdot\bfr'}
\,d\bfr d\bfr'
,
\end{align}
where $\gO$ is the volume of the unit cell,  
and we defined
\begin{align}\label{cn52}
V^\nl(\bfK,\bfK') 
\equiv
\bra{\bfK}
V^\nl
\ket{\bfK'}
=
\frac{1}{\gO}
\int e^{-i\bfK\cdot\bfr}
V^\nl(\bfr,\bfr')
e^{i\bfK'\cdot\bfr'}
\,d\bfr d\bfr'
,
\end{align}
where 
$V^\nl(\bfK',\bfK) =V^{\nl *}(\bfK,\bfK')$, since
$V^\nl(\bfr',\bfr)=V^{\nl*}(\bfr,\bfr')$ due to the fact that $\hat
V^\nl$ is a hermitian operator.
Using the 
plane wave expansion
\begin{align}\label{cn3}
\braket{\bfr}{n\bfk}=\psi_{n\bfk}(\bfr)=\frac{1}{\sqrt{\gO}}
\sum_{\bfG} A_{n\bfk}(\bfG)e^{i\bfK\cdot\bfr}
,
\end{align}
with $\bfK=\bfk+\bfG$, we
obtain from Eq.~\eqref{vnln.0} and Eq.~\eqref{cn51}, that
\begin{align}\label{vnln.2}
\bfv^\nl_{nm}(\bfk)
&=
\frac{i}{\hbar}
\gd(\bfk-\bfk')
\sum_{\bfG,\bfG'}
A^*_{n\bfk}(\bfG) 
A_{m\bfk'}(\bfG')
\frac{1}{\gO}
\int d\bfr d\bfr'
e^{-i\bfK\cdot\bfr}
\bra{\bfr}
[\hat V^\nl,\hat \bfr]
\ket{\bfr'}
e^{i\bfK'\cdot\bfr'}
\nonumber\\
&=
\frac{1}{\hbar}
\gd(\bfk-\bfk')
\sum_{\bfG,\bfG'}
A^*_{n\bfk}(\bfG) 
A_{m\bfk'}(\bfG')
\frac{i}{\gO}
\int d\bfr d\bfr'
e^{-i\bfK\cdot\bfr}
V^\nl(\bfr,\bfr')
\big(\bfr'-\bfr\big)
e^{i\bfK'\cdot\bfr'}
\nonumber\\
&=
\frac{1}{\hbar}
\gd(\bfk-\bfk')
\sum_{\bfG,\bfG'}
A^*_{n\bfk}(\bfG) 
A_{m\bfk'}(\bfG')
(\nabla_\bfK+\nabla_{\bfK'})
V^\nl(\bfK,\bfK')
.
\end{align}  

For fully  separable pseudopotentials in the  
Kleinman-Bylander (KB) form,\cite{mottaCMS10,kleinman_efficacious_1982,adolphPRB96} 
the
matrix elements 
 $\bra{\bfK}
V^\nl
\ket{\bfK'}
=V^\nl(\bfK,\bfK')
$
can be readily calculated. \cite{mottaCMS10}
Indeed,
the Fourier representation assumes 
the form,\cite{adolphPRB96,gordienkoRPJ04,fuchsCPC99}
\begin{align}\label{ji.1} 
V^\nl_{\mathrm{KB}}(\bfK,\bfK')  
 &= 
\sum_s e^{i(\bfK-\bfK')\cdot\bfgtau_s}
\sum_{l=0}^{l_s}\sum_{m=-l}^{l}E_lF_{lm}^s(\bfK)F_{lm}^{s*}(\bfK')  
\nonumber\\
 &= 
\sum_s 
\sum_{l=0}^{l_s}\sum_{m=-l}^{l}E_lf_{lm}^s(\bfK)f_{lm}^{s*}(\bfK')  
,
\end{align} 
with $f^s_{lm}(\bfK)=e^{i\bfK\cdot\bfgtau_s}F^s_{lm}(\bfK)$, and
\begin{align}\label{ji.2}
F^s_{lm}(\bfK)=\int d\bfr\,e^{-i\bfK\cdot\bfr}
\gd V^S_l(\bfr)
\Phi^\ps_{lm}(\bfr) 
.
\end{align}
Here $\gd V^S_l(\bfr)$ is the non-local contribution of the ionic
pseudopotential centered at the atomic position $\bfgtau_s$ located in
the unit cell, 
$\Phi^\ps_{lm}(\bfr)$ is the pseudo-wavefunction of the corresponding
atom, while $E_l$ is the so called 
Kleinman-Bylander energy. Further details can be found in
Ref. \onlinecite{fuchsCPC99}.
From Eq.~\eqref{ji.1} we find
\begin{align}\label{ji.1n}
(\nabla_\bfK+\nabla_{\bfK'})  
V^\nl_{\mathrm{KB}}(\bfK,\bfK') 
 &= 
\sum_s 
\sum_{l=0}^{l_s}\sum_{m=-l}^{l}E_l 
(\nabla_\bfK+\nabla_{\bfK'})   
f_{lm}^s (\bfK)f_{lm}^{s*}(\bfK') 
\nonumber\\
 &= 
\sum_s 
\sum_{l=0}^{l_s}\sum_{m=-l}^{l}E_l 
\left(\left[\nabla_\bfK f_{lm}^s (\bfK)\right]f_{lm}^{s*}(\bfK') 
+
f_{lm}^s (\bfK) \left[\nabla_{\bfK'}  f_{lm}^{s*}(\bfK') \right]
\right),
\end{align}
and using this
 in Eq.~\eqref{vnln.2} leads to
\begin{align}\label{forg}
\bfv^\nl_{nm}(\bfk)
&=
\frac{1}{\hbar}
\sum_s
\sum_{l=0}^{l_s}\sum_{m=-l}^{l}E_l \sum_{\bfG\bfG'}
A^*_{n,\vec{k}}(\bfG)A_{n',\vec{k}}(\bfG')
\nonumber\\
&\times
( \nabla_{\bfK}f_{lm}^s(\bfK)f_{lm}^{s*}(\bfK') +
f_{lm}^s(\bfK)\nabla_{\bfK'}f_{lm}^{s*}(\bfK') ) \nonumber\\
&
=\frac{1}{\hbar}
 \sum_s \sum_{l=0}^{l_s}\sum_{m=-l}^{l}E_l \Bigg[
\Bigg(\sum_{\bfG}A^*_{n,\vec{k}}(\bfG)\nabla_{\bfK}f_{lm}^s(\bfK)\Bigg)
\Bigg(\sum_{\bfG'}A_{n',\vec{k}}(\bfG')
f_{lm}^{s*}(\bfK')\Bigg) \nonumber\\
&+
\Bigg(\sum_{\bfG}A^*_{n,\vec{k}}(\bfG)
f_{lm}^s(\bfK)\Bigg)\Bigg
(\sum_{\bfG'}A_{n',\vec{k}}(\bfG')
\nabla_{\bfK'}f_{lm}^{s*}(\bfK')\Bigg) \Bigg]
,
\end{align}
where there are only single sums over $\bfG$. 
Above is implemented in 
the \depe~code.\cite{francesco}

Indeed, in \depe~\verb=calcolacommutatore.F90= above expansion
coefficients are called\\
 $E_lf_{lm}^s (\bfK)\to$ \verb=fnlkslm= and 
$E_l\nabla_\bfK f_{lm}^s(\bfK)\to$ \verb=fnldkslm=, where 
 \verb=fnlkslm= is an array indexed by $\bfk+\bfG$, and 
 \verb=fnldkslm= is vector  array indexed by $\bfk+\bfG$.

Now we derive $\calbv^{\nl,\ell}_{nm}(\bfk)$. First we prove that
\begin{eqnarray}\label{cvnl.1}
\sum_{\bfG}
\ket{\bfk+\bfG}\bra{\bfk+\bfG}
=1
.
\end{eqnarray}
\noindent Proof:
\begin{align}\label{cvnl.2}
\bra{n\bfk}1\ket{n'\bfk}=\gd_{nn'}
,
\end{align}
take
\begin{align}\label{cvnl.3}
\sum_\bfG \bra{n\bfk}\ket{\bfk+\bfG}\bra{\bfk+\bfG}\ket{n'\bfk}
&=
\int d\bfr d\bfr' 
\sum_\bfG \bra{n\bfk}
\ket{\bfr}\bra{\bfr}
\ket{\bfk+\bfG}\bra{\bfk+\bfG}
\ket{\bfr'}\bra{\bfr'}
\ket{n'\bfk}
\nonumber\\
&=
\int d\bfr d\bfr' 
\sum_\bfG 
\psi^*_{n\bfk}(\bfr) 
\frac{1}{\sqrt{\gO}}e^{i(\bfk+\bfG)\cdot\bfr}
\frac{1}{\sqrt{\gO}}e^{-i(\bfk+\bfG)\cdot\bfr'}
\psi_{m\bfk}(\bfr') 
\nonumber\\
&=
\int d\bfr d\bfr' 
\psi^*_{n\bfk}(\bfr) 
\psi_{m\bfk}(\bfr') 
\frac{1}{V}
\sum_\bfG 
e^{i(\bfk+\bfG)\cdot(\bfr-\bfr')}
\nonumber\\
&=
\int d\bfr d\bfr' 
\psi^*_{n\bfk}(\bfr) 
\psi_{m\bfk}(\bfr') 
\gd(\bfr-\bfr')
=
\int d\bfr
\psi^*_{n\bfk}(\bfr) 
\psi_{m\bfk}(\bfr)=\gd_{nn'} ,
\end{align}
and thus Eq.~\eqref{cvnl.1} follows. \verb=Q.E.D.=
We used
\begin{align}\label{vnl.4}
\braket{\bfr}{\bfk+\bfG}=\frac{1}{\sqrt{\gO}}e^{i(\bfk+\bfG)\cdot\bfr}
.
\end{align}

From Eq.~\eqref{nl.4}, we would like to calculate
\begin{align}\label{vnl.5}
\calbv^{\nl,\ell}_{nm}(\bfk)=\frac{1}{2}
\bra{n\bfk} 
C^\ell(z)\bfv^\nl+\bfv^\nl C^\ell(z)  
\ket{m\bfk}
.
\end{align}  
We work out the first term in the r.h.s,
\begin{align}\label{vnl.6}
\bra{n\bfk}C^\ell(z) 
\bfv^\nl\ket{m\bfk}
&=\sum_{\bfG}
\bra{n\bfk}C^\ell(z)\ket{\bfk+\bfG}
\bra{\bfk+\bfG}\bfv^\nl\ket{m\bfk}
\nonumber\\
&=\sum_{\bfG}
\int d\bfr 
\int d\bfr' 
\bra{n\bfk}
\ket{\bfr}\bra{\bfr}  
C^\ell(z) 
\ket{\bfr'}\bra{\bfr'}
\ket{\bfk+\bfG}
\nonumber\\
&\times 
\int d\bfr'' 
\int d\bfr''' 
\bra{\bfk+\bfG}
\ket{\bfr''}\bra{\bfr''} 
\bfv^\nl 
\ket{\bfr'''}\bra{\bfr'''} 
\ket{m\bfk}
\nonumber\\
&=\sum_{\bfG}
\int d\bfr 
\int d\bfr' 
\braket{n\bfk}{\bfr}
C^\ell(z) 
\gd(\bfr-\bfr') 
\braket{\bfr'}{\bfk+\bfG}
\nonumber\\
&\times 
\int d\bfr'' 
\int d\bfr''' 
\braket{\bfk+\bfG}{\bfr''}
\bra{\bfr''} 
\bfv^\nl 
\ket{\bfr'''}
\braket{\bfr'''}{m\bfk}
\nonumber\\
&=\sum_{\bfG}
\int d\bfr 
\braket{n\bfk}{\bfr}
C^\ell(z) 
\braket{\bfr}{\bfk+\bfG}
\nonumber\\
&\times 
\frac{i}{\hbar}
\int d\bfr'' 
\int d\bfr''' 
\braket{\bfk+\bfG}{\bfr''}
V^\nl(\bfr'',\bfr''')(\bfr'''-\bfr'') 
\braket{\bfr'''}{m\bfk}
,
\end{align}
where we used Eq.~\eqref{vnln.1} and \eqref{conhr}. 
We use Eq.~\eqref{cn3}, \eqref{vnl.4} and \eqref{cn51}  to obtain
\begin{align}\label{vnl.7}
\bra{n\bfk}C^\ell(z) 
\bfv^\nl\ket{m\bfk}
&=\sum_{\bfG}
\sum_{\bfG'}
A^*_{n\bfk}(\bfG') 
\frac{1}{\gO}
\int d\bfr 
e^{-i(\bfk+\bfG')\cdot\bfr}
C^\ell(z) 
e^{i(\bfk+\bfG)\cdot\bfr}
\nonumber\\
&\times 
\sum_{\bfG''}
A_{m\bfk}(\bfG'') 
\frac{i}{\hbar\gO}
\int d\bfr'' 
\int d\bfr''' 
e^{-i(\bfk+\bfG)\cdot\bfr''} 
V^\nl(\bfr'',\bfr''')(\bfr'''-\bfr'') 
e^{i(\bfk+\bfG'')\cdot\bfr'''}
\nonumber\\
&=
\frac{1}{\hbar}
\sum_{\bfG}
\sum_{\bfG'}
A^*_{n\bfk}(\bfG') 
\gd_{\bfG_\parallel \bfG'_\parallel}f_\ell(\bfG_\perp-\bfG'_\perp) 
\sum_{\bfG''}
A_{m\bfk}(\bfG'') 
(\nabla_{\bfK}+\nabla_{\bfK''}) 
V^\nl(\bfK,\bfK'') 
,
\end{align}
where
\begin{align}\label{vnl.8}
\frac{1}{\gO}
\int d\bfr\, 
C^\ell(z) 
e^{i(\bfG-\bfG')\cdot\bfr}
=\gd_{\bfG_\parallel \bfG'_\parallel}f_\ell(\bfG_\perp-\bfG'_\perp)
,
\end{align} 
and
\begin{align}\label{vnl.9}
f_\ell(g)=\frac{1}{L}\int_{z_\ell-\gD^b_\ell}^{z_\ell+\gD^f_\ell} e^{igz}dz  
 ,
\end{align}
where $f^*(g)=f(-g)$.
We define
\begin{align}\label{vnl.10}
\calf^\ell_{n\bfk}(\bfG) 
=
\sum_{\bfG'}
A_{n\bfk}(\bfG') 
\gd_{\bfG_\parallel \bfG'_\parallel}f_\ell(\bfG'_\perp-\bfG_\perp) 
,
\end{align}
and
\begin{align}\label{vnl.11}
\calh_{n\bfk}(\bfG)&=
\sum_{\bfG'}
A_{n\bfk}(\bfG') 
(\nabla_{\bfK}+\nabla_{\bfK'}) 
V^\nl(\bfK,\bfK') 
,
\end{align}
thus we can compactly write,
\begin{align}\label{vn.12}
\bra{n\bfk}C^\ell(z) 
\bfv^\nl\ket{m\bfk}
&=
\frac{1}{\hbar}
\sum_{\bfG}
\calf^{\ell*}_{n\bfk}(\bfG) 
\calh_{m\bfk}(\bfG) 
.
\end{align}
Now, the second term of Eq.~\eqref{vnl.5}
\begin{align}\label{vnl.12}
\bra{n\bfk}
\bfv^\nl
C^\ell(z) \ket{m\bfk}
&=\sum_{\bfG}
\bra{n\bfk}
\bfv^\nl 
\ket{\bfk+\bfG}
\bra{\bfk+\bfG}C^\ell(z)
\ket{m\bfk}
\nonumber\\
&=\sum_{\bfG}
\int d\bfr'' 
\int d\bfr''' 
\bra{n\bfk}
\ket{\bfr''}\bra{\bfr''} 
\bfv^\nl 
\ket{\bfr'''}\bra{\bfr'''} 
\ket{\bfk+\bfG}
\nonumber\\
&\times 
\int d\bfr 
\int d\bfr' 
\bra{\bfk+\bfG}
\ket{\bfr}\bra{\bfr}  
C^\ell(z) 
\ket{\bfr'}\bra{\bfr'}
\ket{m\bfk}
\nonumber\\
&=\sum_{\bfG}
\frac{i}{\hbar}
\int d\bfr'' 
\int d\bfr''' 
\braket{n\bfk}{\bfr''}
V^\nl(\bfr'',\bfr''')(\bfr'''-\bfr'') 
\braket{\bfr'''}{\bfk+\bfG}
\nonumber\\
&\times 
\int d\bfr 
\braket{\bfk+\bfG}{\bfr}
C^\ell(z) 
\braket{\bfr}{m\bfk}
\nonumber\\
&=\sum_{\bfG}
\sum_{\bfG'}
A^*_{n\bfk}(\bfG') 
\frac{i}{\hbar\gO}
\int d\bfr'' 
\int d\bfr''' 
e^{-i(\bfk+\bfG')\cdot\bfr''} 
V^\nl(\bfr'',\bfr''')(\bfr'''-\bfr'') 
e^{i(\bfk+\bfG)\cdot\bfr'''}
\nonumber\\
&\times 
\sum_{\bfG''}
A_{m\bfk}(\bfG'') 
\frac{1}{\gO}
\int d\bfr 
e^{-i(\bfk+\bfG)\cdot\bfr} 
C^\ell(z) 
e^{i(\bfk+\bfG'')\cdot\bfr}
\nonumber\\
&=
\frac{1}{\hbar}
\sum_{\bfG}
\sum_{\bfG'}
A^*_{n\bfk}(\bfG') 
(\nabla_\bfK+\nabla_{\bfK'})
V^\nl(\bfK',\bfK)
\nonumber\\
&\times 
\sum_{\bfG''}
A_{m\bfk}(\bfG'') 
\gd_{\bfG_\parallel \bfG''_\parallel}f_\ell(\bfG''_\perp-\bfG_\perp)
\nonumber\\
&=
\frac{1}{\hbar}
\sum_{\bfG}
\calh^*_{n\bfk}(\bfG) 
\calf^\ell_{m\bfk}(\bfG) 
.
\end{align}
Therefore Eq.~\eqref{vnl.5} is compactly given by
\begin{align}\label{vnl.13}
\calbv^{\nl,\ell}_{nm}(\bfk)=\frac{1}{2 \hbar}
\sum_{\bfG}
\left(
\calf^{\ell*}_{n\bfk}(\bfG) 
\calh_{m\bfk}(\bfG) 
+
\calh^*_{n\bfk}(\bfG) 
\calf^\ell_{m\bfk}(\bfG) 
\right)
.
\end{align} 
For fully  separable pseudopotentials in the 
Kleinman-Bylander (KB) form,\cite{mottaCMS10,kleinman_efficacious_1982,adolphPRB96}
we can use Eq.~\eqref{ji.1n} and evaluate above expression, that we have
implemented in 
the \depe~code.\cite{francesco}
Explicitly,
\begin{eqnarray}\label{vnl.14}
\calbv^{\nl,\ell}_{nm}(\bfk)=\frac{1}{2 \hbar}
\sum_s\sum_{l=0}^{l_s}\sum_{m=-l}^{l}E_l \nonumber\\
\Bigg[ \Bigg(\sum_{{\bfG''}}
\nabla_{{\bfG''}}f_{lm}^s({\bfG''})
\sum_{\bfG}A^*_{n{\bfk}}(\bfG)\delta_{\bfG_{||}{\bfG''}_{||}}
f_\ell(G_z-G''_z) \Bigg)  
\Bigg( \sum_{{\bfG'}}A_{m{\bfk}}({\bfG'})f_{lm}^{s*}({\bfK'}) \Bigg) \nonumber\\
%
+ \Bigg(\sum_{{\bfG''}}
f_{lm}^s({\bfG''})\sum_{\bfG}A^*_{n{\bfk}}(\bfG)\delta_{\bfG_{||}{\bfG''}_{||}}
f_\ell(G_z-G''_z) \Bigg)  
\Bigg( \sum_{{\bfG'}}A_{m{\bfk}}({\bfG'})\nabla_{{\bfK'}}f_{lm}^{s*}({\bfK'}) \Bigg)  \nonumber\\
+
\Bigg(\sum_{\bfG}A^*_{n{\bfk}}(\bfG)\nabla_{\bfG}f_{lm}^s(\bfG)\Bigg)\Bigg(
\sum_{{\bfG''}}
f_{lm}^{s*}({\bfG''})\sum_{{\bfG'}}A_{m{\bfk}}({\bfG'})\delta_{{\bfG'}_{||}{\bfG''}_{||}}
f_\ell(G''_z-G'_z) \Bigg) \nonumber\\ 
+
\Bigg(\sum_{\bfG}A^*_{n{\bfk}}(\bfG)f_{lm}^s(\bfG)
\Bigg) \Bigg(
\sum_{{\bfG''}}\nabla_{{\bfG''}}f_{lm}^{s*}({\bfG''})
\sum_{{\bfG'}}A_{m{\bfk}}({\bfG'})\delta_{{\bfG'}_{||}{\bfG''}_{||}}
f_\ell(G''_z-G'_z) \Bigg) \Bigg].\nonumber\\ 
\end{eqnarray} 
For a full slab calculation, equivalent to a bulk calculation,
$C^\ell(z)=1$ and then 
$f_\ell(g) =\gd_{g0}$, and Eq.~\eqref{vnl.14}
reduces to 
Eq.~\eqref{forg}. 

